\documentclass[10pt,a4paper]{article}
\usepackage[utf8]{inputenc}
\usepackage{mathtools}
\usepackage{amsfonts}
\usepackage{amssymb}
\usepackage{graphicx}
\author{Stanley}
\title{tutorial}
\begin{document}
Writing $x=2$ is equivalent to $x-2 = 0$
khgi jskhfguir jkhgur jkhgri jhriu hgeoiru jrhoiuh \eqref{eqn1} shows thatabove $x=2$

	Writing $$x=2$$ is equivalent to $x-2 = 0$  a$\leq$x$\geq$b

\begin{equation}\label{eqn1}
x=2
\end{equation}

\begin{eqnarray}
0&=&x+y \label{sys1}\\ 0=x+y \\
2 &=& x-y \label{sys2}
\end{eqnarray}

\begin{eqnarray*}
	0&=&x+y \label{sys1}\\ 0=x+y \\
	2 &=& x-y \label{sys2} 2 = x-y
\end{eqnarray*}


$$\frac{x}{y}$$



$$\sum_{i=1}^{n}=$$

$$\sum_{i=1}^n i^3= \left( \frac{n(n+1)}{2}\right)^{2} $$


$$\int \frac{d\theta}{\theta^{2}+1}=\tan^{-1}\theta+c$$

$$x^{2}+\frac{b}{a}x=-\frac{c}{a}+\left(\frac{b}{2a}\right)^{2}$$

$$\left(x+\frac{b}{2a}\right)^{2}=-\frac{c}{d}+\frac{b^{2}}{4a^{2}}$$

$$\left(x+\frac{b}{2a}\right)^{2}=\frac{b^{2}-4ac}{4a^{2}}$$
$$\sum_{k=1}^{\frac{a}{2}-1}\frac{\prod_{n=0}^{k-1}\left(6-2n\right)}{\prod_{n=0}}^{k \left(6-2n+1\right)}+\frac{1}{a+1}$$
$$\sum_{k=1}^{\frac{a}{2}-1}\frac{\displaystyle\prod_{n=0}^{k-1}\left(6-2n\right)}{\displaystyle\prod_{n=0}^{k}\left(6-2n+1\right)}+\frac{1}{a+1}$$

First, suppose that D is a region of  that is, it can be described by inequalities a$\leq$x$\geq$b and where $\gamma$ and $\delta$ are  where functions First, weâ€™ll show that
\end{document}